x86model/Model/BiGrammar.v
@@ -1,0 +1,496 @@
+(** Gang Tan: Bi-directional grammars for both parsing and pretty-printing *)
+
+Require Import Coq.Program.Equality.
+Require Import Coq.Init.Logic.
+Require Import Coqlib.  (* for extensionality & proof_irrelevance *)
+Require Import Arith.
+Require Import Eqdep.
+Require Import Omega.
+Require Import CommonTacs.
+Require Import Program.
+
+Unset Automatic Introduction. 
+Set Implicit Arguments.
+
+Require Import Monad.
+Local Open Scope monad_scope.
+
+Require Import ParserArg.
+
+(* Module Type NEW_PARSER_ARG. *)
+(*   (* the type of characters used in the grammar specifications *) *)
+(*   Parameter char_p : Set. *)
+(*   (* equality on characters -- should change this to a boolean function, *)
+(*      paired with a proof that it's an equality so that *)
+(*      we get faster symbolic computation. *) *)
+(*   Parameter char_dec : forall (c1 c2:char_p), {c1=c2} + {c1<>c2}. *)
+(*   (* a name for user types embedded within our AST grammar types. *) *)
+(*   Parameter user_type : Set. *)
+(*   (* equality on user type names. *) *)
+(*   Parameter user_type_dec : forall (t1 t2:user_type), {t1=t2} + {t1<>t2}. *)
+(*   (* a semantic interpretation function for user type names. *) *)
+(*   Parameter user_type_denote : user_type -> Set. *)
+
+(*   (* when we parse, instead of working in terms of individual characters, *)
+(*      we work in terms of tokens.   For instance, the x86 grammar is specified *)
+(*      with characters as bits, and tokens as bytes (8-bits. *) *)
+(*   Definition token_id := nat. *)
+(*   (* this is the total number of tokens that we can have -- e.g., for the *)
+(*      x86 parser it is 256 because they have 8 bits. *) *)
+(*   Variable num_tokens : nat. *)
+(*   (* this converts tokens to a list of characters -- it's used only during *)
+(*      the table construction for the parser. *) *)
+(*   Variable token_id_to_chars : token_id -> list char_p. *)
+(* End NEW_PARSER_ARG. *)
+
+(* a module for generating the parser for x86 instructions *)
+(* Module X86_PARSER_ARG. *)
+(*   Require Import X86Syntax. *)
+(*   Require Import Bits. *)
+(*   Local Open Scope Z_scope. *)
+  
+(*   Definition char_p : Set := bool. *)
+(*   Definition char_dec : forall (c1 c2:char_p), {c1=c2}+{c1<>c2} := bool_dec. *)
+(*   Inductive type : Set :=  *)
+(*   | Int_t : type *)
+(*   | Register_t : type *)
+(*   | BitVector_t : nat -> type (* a bit vector of a certain width *) *)
+(*   (* | Byte_t : type *) *)
+(*   (* | Half_t : type *) *)
+(*   (* | Word_t : type *) *)
+(*   (* | Double_Word_t : type *) *)
+(*   (* | Ten_Byte_t : type *) *)
+(*   | Scale_t : type *)
+(*   | Condition_t : type *)
+(*   | Address_t : type *)
+(*   | Operand_t : type *)
+(*   | Fpu_Register_t : type *)
+(*   | Fp_Debug_Register_t : type *)
+(*   | Fp_Operand_t : type  *)
+(*   | MMX_Granularity_t : type *)
+(*   | MMX_Register_t : type *)
+(*   | MMX_Operand_t : type *)
+(*   | SSE_Register_t : type *)
+(*   | SSE_Operand_t : type *)
+(*   | Instruction_t : type *)
+(*   | Control_Register_t : type *)
+(*   | Debug_Register_t : type *)
+(*   | Segment_Register_t : type *)
+(*   | Lock_or_Rep_t : type *)
+(*   | Bool_t : type *)
+(*   | Prefix_t : type *)
+(*   | Option_t (t: type) : type *)
+(*   (* Need pairs at this level if I want to have options of pairs*) *)
+(*   | UPair_t (t1 t2: type) : type.  *)
+
+(*   Definition Byte_t := BitVector_t 7. *)
+(*   Definition Half_t := BitVector_t 15. *)
+(*   Definition Word_t := BitVector_t 31. *)
+(*   Definition Double_Word_t := BitVector_t 63. *)
+(*   Definition Ten_Byte_t := BitVector_t 79. *)
+
+(*   Definition tipe := type. *)
+(*   Definition tipe_eq : forall (t1 t2:tipe), {t1=t2} + {t1<>t2}. *)
+(*     intros ; decide equality. *)
+(*     apply eq_nat_dec. *)
+(*   Defined. *)
+
+(*   Fixpoint tipe_m (t:tipe) :=  *)
+(*     match t with  *)
+(*       | Int_t => Z *)
+(*       | Register_t => register *)
+(*       | BitVector_t n => Word.int n *)
+(*       (* | Byte_t => int8 *) *)
+(*       (* | Half_t => int16 *) *)
+(*       (* | Word_t => int32 *) *)
+(*       (* | Double_Word_t => int64 *) *)
+(*       (* | Ten_Byte_t => int80 *) *)
+(*       | Scale_t => scale *)
+(*       | Condition_t => condition_type *)
+(*       | Address_t => address *)
+(*       | Operand_t => operand *)
+(*       | Fpu_Register_t => int3 *)
+(*       | Fp_Debug_Register_t => fp_debug_register *)
+(*       | Fp_Operand_t => fp_operand   *)
+(*       | MMX_Granularity_t => mmx_granularity *)
+(*       | MMX_Register_t => mmx_register *)
+(*       | MMX_Operand_t => mmx_operand *)
+(*       | SSE_Register_t => sse_register *)
+(*       | SSE_Operand_t => sse_operand *)
+(*       | Instruction_t => instr *)
+(*       | Control_Register_t => control_register *)
+(*       | Debug_Register_t => debug_register *)
+(*       | Segment_Register_t => segment_register *)
+(*       | Lock_or_Rep_t => lock_or_rep *)
+(*       | Bool_t => bool *)
+(*       | Prefix_t => prefix *)
+(*       | Option_t t => option (tipe_m t) *)
+(*       | UPair_t t1 t2 => ((tipe_m t1) * (tipe_m t2))%type *)
+(*     end. *)
+(*   Definition user_type := type. *)
+(*   Definition user_type_dec : forall (t1 t2:user_type), {t1=t2} + {t1<>t2} :=  *)
+(*     tipe_eq. *)
+(*   Definition user_type_denote := tipe_m. *)
+
+(*   Definition byte_explode (b:int8) : list bool :=  *)
+(*   let bs := Word.bits_of_Z 8 (Word.unsigned b) in *)
+(*     (bs 7)::(bs 6)::(bs 5)::(bs 4)::(bs 3)::(bs 2)::(bs 1)::(bs 0)::nil. *)
+
+(*   Definition nat_explode (n:nat) : list bool :=  *)
+(*     byte_explode (Word.repr (Z_of_nat n)). *)
+
+(*   Definition token_id := nat. *)
+(*   Definition num_tokens : token_id := 256%nat. *)
+(*   Definition token_id_to_chars : token_id -> list char_p := nat_explode. *)
+(* End X86_PARSER_ARG. *)
+
+Definition char_p := X86_PARSER_ARG.char_p.
+Definition char_dec := X86_PARSER_ARG.char_dec.
+Definition user_type := X86_PARSER_ARG.user_type.
+Definition user_type_dec := X86_PARSER_ARG.user_type_dec.
+Definition user_type_denote := X86_PARSER_ARG.user_type_denote.
+Definition token_id := X86_PARSER_ARG.token_id.
+Definition num_tokens := X86_PARSER_ARG.num_tokens.
+Definition token_id_to_chars := X86_PARSER_ARG.token_id_to_chars.
+
+
+(** The [type]s for our grammars. *)
+Inductive type : Type := 
+| Unit_t : type
+| Char_t : type
+| Void_t : type
+| Pair_t : type -> type -> type
+| Sum_t : type -> type -> type
+| List_t : type -> type
+| User_t : user_type -> type.
+
+(** [void] is an empty type. *)
+Inductive void : Type := .
+
+(** The interpretation of [type]s as Coq [Type]s. *)
+Fixpoint interp (t:type) : Type := 
+  match t with 
+    | Unit_t => unit
+    | Char_t => char_p
+    | Void_t => void
+    | Pair_t t1 t2 => (interp t1) * (interp t2)
+    | Sum_t t1 t2 => (interp t1) + (interp t2)
+    | List_t t => list (interp t)
+    | User_t t => user_type_denote t
+  end%type.
+
+(* notation [[ t ]] would interfere with "destruct H as [v [H2 H4]]" *)
+Notation "[| t |]" := (interp t).
+
+(** a pair of a function and its inverse *)
+Notation funinv t1 t2 := (([|t1|] -> [|t2|]) * 
+                          ([|t2|] -> option ([|t1|])))%type.
+
+(** Bi-directional grammars, which are used to generate parsers and pretty printers. *)
+(** Our user-facing [grammar]s, indexed by a [type], reflecting the type of the
+    semantic value returned by the grammar when used in parsing. *)
+(** After erasing the pretty-print functions, we can go easily from a bi-directional grammar 
+    to a regular grammar that specifies parsing. 
+    We can perform optimizations on regular grammars as usual. It seems we should
+    avoid optimizations on bi-directional grammars, which requires adjustments on 
+    both parse and pretty-print functions.
+*)
+
+Inductive bigrammar : type -> Type := 
+| Eps : bigrammar Unit_t
+| Zero : forall t, bigrammar t
+| Char : char_p -> bigrammar Char_t
+| Any : bigrammar Char_t
+| Cat : forall t1 t2, bigrammar t1 -> bigrammar t2 -> bigrammar (Pair_t t1 t2)
+| Alt : forall t1 t2, bigrammar t1 -> bigrammar t2 -> bigrammar (Sum_t t1 t2)
+(* todo: add Star back *)
+(* | Star : forall t, bigrammar t -> bigrammar (List_t t) *)
+| Map : forall t1 t2
+          (fi: (funinv t1 t2)), (* a parse function and a pretty print function *)
+          bigrammar t1 -> bigrammar t2.
+Implicit Arguments Map [t1 t2].
+
+(** Denotation of Bi-Grammars *)
+(** I'm a little annoyed that I had to break out so many equalities, but
+    found this worked a little better for both inversion and proving. *)
+Inductive in_bigrammar : forall t, bigrammar t -> list char_p -> (interp t) -> Prop := 
+| InEps : forall s v, s = nil -> v = tt -> in_bigrammar Eps s v
+| InChar : forall c s v, s = c::nil -> v = c -> in_bigrammar (Char c) s v
+| InAny : forall c s v, s = c::nil -> v = c -> in_bigrammar Any s v
+| InCat : forall t1 t2 (g1:bigrammar t1) (g2:bigrammar t2) s1 s2 v1 v2 s v, 
+    in_bigrammar g1 s1 v1 -> in_bigrammar g2 s2 v2 -> 
+    s = s1 ++ s2 -> v = (v1,v2) -> in_bigrammar (Cat g1 g2) s v
+| InAlt_l : forall t1 t2 (g1:bigrammar t1) (g2:bigrammar t2) s v1 v, 
+    in_bigrammar g1 s v1 -> v = inl _ v1 -> in_bigrammar (Alt g1 g2) s v
+| InAlt_r : forall t1 t2 (g1:bigrammar t1) (g2:bigrammar t2) s v2 v, 
+    in_bigrammar g2 s v2 -> v = inr _ v2 -> in_bigrammar (Alt g1 g2) s v
+(* | InStar_eps : forall t (g:bigrammar t) s v, s = nil -> v = nil -> in_bigrammar (Star g) s v *)
+(* | InStar_cons : forall t (g:bigrammar t) s1 v1 s2 v2 s v,  *)
+(*     in_bigrammar g s1 v1 -> in_bigrammar (Star g) s2 v2 ->  *)
+(*     s1 <> nil -> s = s1 ++ s2 -> v = v1::v2 -> in_bigrammar (Star g) s v *)
+| InMap : forall t1 t2 (fi:funinv t1 t2) (g:bigrammar t1) s v1 v2, 
+    in_bigrammar g s v1 -> v2 = fst fi v1 -> in_bigrammar (@Map t1 t2 fi g) s v2.
+Hint Constructors in_bigrammar.
+
+(** Explicit inversion principles for the grammars -- needed because
+    of typing dependencies, though a little awkward that we can't just
+    use [dependent inversion] to solve them. *)
+Lemma EpsInv : forall cs v, in_bigrammar Eps cs v -> cs = nil /\ v = tt.
+  intros. inversion H; crush.
+Qed.
+Lemma AnyInv : forall cs v, in_bigrammar Any cs v -> cs = v::nil.
+  intros. inversion H ; subst ; crush.
+Qed.
+Lemma CharInv : forall c cs v, in_bigrammar (Char c) cs v -> cs = c::nil /\ v = c.
+  intros. inversion H ; subst ; crush.
+Qed.
+Lemma CatInv : forall t1 t2 (g1:bigrammar t1) (g2:bigrammar t2) cs v, 
+  in_bigrammar (Cat g1 g2) cs v -> 
+  exists cs1, exists cs2, exists v1, exists v2, 
+    in_bigrammar g1 cs1 v1 /\ in_bigrammar g2 cs2 v2 /\ cs = cs1++cs2 /\ v = (v1,v2).
+Proof.
+  intros. inversion H ; subst ; crush. eauto 8.
+Qed.
+Lemma AltInv : forall t1 t2 (g1:bigrammar t1) (g2:bigrammar t2) cs v, 
+  in_bigrammar (Alt g1 g2) cs v -> 
+  (exists v1, in_bigrammar g1 cs v1 /\ v = inl _ v1) \/
+  (exists v2, in_bigrammar g2 cs v2 /\ v = inr _ v2).
+Proof.
+  intros ; inversion H ; subst ; crush; eauto.
+Qed.
+ (*Lemma StarInv : forall t (g:bigrammar t) cs v,  
+   in_bigrammar (Star g) cs v -> (cs = nil /\ v = nil) \/  
+   (exists cs1, exists v1, exists cs2, exists v2,  
+     cs1 <> nil /\ in_bigrammar g cs1 v1 /\ in_bigrammar (Star g) cs2 v2 /\  
+    cs = cs1 ++ cs2 /\ v = v1::v2).
+ Proof. 
+   intros ; inversion H ; clear H ; subst ; mysimp ; right ; exists s1 ; exists v1 ;  
+   exists s2 ; exists v2 ; auto. 
+ Qed. *)
+Lemma MapInv : forall t1 t2 (fi: funinv t1 t2) (g:bigrammar t1) cs v,
+  in_bigrammar (@Map t1 t2 fi g) cs v -> exists v', in_bigrammar g cs v' /\ v = fst fi v'.
+Proof.
+  intros ; inversion H ; subst ; crush. 
+Qed.
+Lemma ZeroInv : forall t cs v, in_bigrammar (Zero t) cs v -> False.
+  intros ; inversion H.
+Qed.
+(*
+Lemma XformInv : forall t1 t2 (x:t1->>t2) (g:grammar t1) cs v,
+  in_bigrammar (Xform x g) cs v -> exists v', in_bigrammar g cs v' /\ v = xinterp x v'.
+Proof.
+  intros ; inversion H ; mysimp. exists v1. auto.
+Qed.
+*)
+
+(** Tactic for invoking inversion principles on a proof that some string
+    and value are in the denotation of a grammar.  We don't unroll the 
+    [Star] case because that would loop. *)
+Ltac in_bigrammar_inv := 
+  repeat 
+    match goal with 
+      | [ H : in_bigrammar Eps _ _ |- _ ] => generalize (EpsInv H) ; clear H
+      | [ H : in_bigrammar Any _ _ |- _ ] => generalize (AnyInv H) ; clear H
+      | [ H : in_bigrammar (Char _) _ _ |- _ ] => generalize (CharInv H) ; clear H
+      | [ H : in_bigrammar (Alt _ _) _ _ |- _ ] => generalize (AltInv H) ; clear H
+      | [ H : in_bigrammar (Cat _ _) _ _ |- _ ] => generalize (CatInv H) ; clear H
+      | [ H : in_bigrammar (Zero _) _ _ |- _ ] => contradiction (ZeroInv H)
+      | [ H : in_bigrammar (Map _ _) _ _ |- _ ] => generalize (MapInv H) ; clear H
+      | _ => idtac
+    end.
+
+Definition in_bigrammar_rng t (g: bigrammar t) (v: interp t) := 
+  exists s, in_bigrammar g s v.
+
+Definition bigrammar_rng_subset t1 t2 (g1: bigrammar t1) (f: interp t1 -> interp t2)
+           (g2: bigrammar t2) := 
+  forall v1, in_bigrammar_rng g1 v1 -> in_bigrammar_rng g2 (f v1).
+
+Definition invertible t1 t2 (fi: funinv t1 t2) (g:bigrammar t1) :=
+  (forall v: [|t1|],
+     in_bigrammar_rng g v ->
+     (* need the second conjunct to prove pretty_print_corr1 for the map case *)
+     (exists v', (snd fi) (fst fi v) = Some v' /\ in_bigrammar_rng g v')) /\
+  (forall (v:[|t1|]) (w:[|t2|]),
+     in_bigrammar_rng g v -> snd fi w = Some v -> fst fi v = w).
+Implicit Arguments invertible [t1 t2].
+
+(** compose two pairs of functions and inverses *)
+Definition funinv_compose t1 t2 t3 (fi2: funinv t2 t3) (fi1: funinv t1 t2) :=
+  (compose (fst fi2) (fst fi1), 
+   fun w => match snd fi2 w with
+              | None => None
+              | Some u => snd fi1 u
+            end).
+Implicit Arguments funinv_compose [t1 t2 t3].
+
+
+(* The following version of invertible uses subset types to simplify the
+   definition, but I found it's difficult to work this definition with
+   tactics; whenever there is a value of the subset type, I need to
+   destruct that value.
+*)
+(* Notation in_rng_val t g := {v:t | in_bigrammar_rng g v}. *)
+(* Definition invertible t1 t2 (f:interp t1 -> interp t2)  *)
+(*              (finv:interp t2 -> option (interp t1)) (g:bigrammar t1) :=  *)
+(*   (forall v: in_rng_val _ g, *)
+(*      exists v': in_rng_val _ g, finv (f (` v)) = Some (` v')) /\ *)
+(*   (forall (v: in_rng_val _ g) (w:interp t2),  *)
+(*      finv w = Some (` v) -> f (` v) = w). *)
+
+(* well-formedness of grammars *)
+Fixpoint wf_grammar t (g:bigrammar t) : Prop := 
+  match g with 
+      | Cat t1 t2 g1 g2 => wf_grammar g1 /\ wf_grammar g2
+      | Alt t1 t2 g1 g2 => wf_grammar g1 /\ wf_grammar g2
+      (* | Star t g => wf_grammar g *)
+      | Map t1 t2 fi g => 
+        wf_grammar g /\ invertible fi g
+      | g' => True
+  end.
+
+(* a well-formed bigrammar: a bigrammar with a proof that it is well-formed *)
+Notation wf_bigrammar t := {g:bigrammar t | wf_grammar g}.
+
+(********************************* Pretty Printer *************************************)
+
+Fixpoint pretty_print t (g:bigrammar t) : interp t -> option (list char_p) :=
+  match g in bigrammar t' return interp t' -> option (list char_p) with
+    | Eps => fun v => Some nil
+    | Char c => fun c' => if char_dec c c' then Some (c::nil) else None
+    | Any => fun c => Some (c::nil)
+    | Zero t => fun impos => None
+    | Cat t1 t2 g1 g2 =>
+      fun p =>
+        s1 <- pretty_print g1 (fst p);
+        s2 <- pretty_print g2 (snd p);
+        ret (s1 ++ s2)
+    | Alt t1 t2 g1 g2 =>
+      fun v => match v with
+                 | inl x1 => pretty_print g1 x1
+                 | inr x2 => pretty_print g2 x2
+               end
+    (* | Star t g => *)
+    (*   (* this is a non-tail-recusive version, which is easier to prover *) *)
+    (*   fix loop (v:interp (List_t t)) : option (list char_p) := *)
+    (*      match v with *)
+    (*        | nil => Some nil *)
+    (*        | hd::tl => *)
+    (*          s' <- pretty_print g hd; *)
+    (*          match s' with *)
+    (*            | nil => None (* g cannot match the empty input list *) *)
+    (*            | _ => s <- loop tl; ret s' ++ s *)
+    (*          end *)
+    (*      end *)
+    (*   (* (fix loop (s : list char_p)(v:interp (List_t t)) : option (list char_p) := *) *)
+    (*   (*    match v with *) *)
+    (*   (*      | nil => Some s *) *)
+    (*   (*      | hd::tl => *) *)
+    (*   (*        s' <- pretty_print g hd; *) *)
+    (*   (*        match s' with *) *)
+    (*   (*          | nil => None (* g cannot match the empty input list *) *) *)
+    (*   (*          | _ => loop (s ++ s') tl *) *)
+    (*   (*        end *) *)
+    (*   (*    end) nil *) *)
+    | Map t1 t2 fi g =>
+      fun v => x <- snd fi v; pretty_print g x
+  end.
+
+Local Ltac localsimpl :=
+  repeat
+    match goal with
+      | [v: unit |- _ ] => destruct v
+      | [ |- context[char_dec ?x ?y] ] => destruct (char_dec x y)
+      | [_: context[char_dec ?x ?y] |- _] => destruct (char_dec x y)
+      | [H: wf_bigrammar _ |- _] => destruct H
+      | _ => unfold invertible, in_bigrammar_rng in *; in_bigrammar_inv; crush
+    end.
+
+Lemma in_bigrammar_rng_map t1 t2 (g:bigrammar t1) (fi: funinv t1 t2) v:
+  in_bigrammar_rng g v -> in_bigrammar_rng (Map fi g) (fst fi v).
+Proof. unfold in_bigrammar_rng; crush. Qed.
+
+(* Ltac guess_in_all v := *)
+(*   match goal with  *)
+(*     | [H: forall x: ?T, _ |- _] => *)
+(*       match type of v with *)
+(*         | T => guess v H *)
+(*       end *)
+(*   end. *)
+      
+Lemma compose_invertible
+      t1 t2 t3 (g:bigrammar t1) (fi1:funinv t1 t2) (fi2: funinv t2 t3):
+      invertible fi1 g -> invertible fi2 (Map fi1 g) ->
+      invertible (funinv_compose fi2 fi1) g.
+Proof. unfold invertible; intros; breakHyp; simpl; unfold compose.
+  split; intros;
+  use_lemma (@in_bigrammar_rng_map _ _ g fi1) by eassumption.
+  - match goal with
+      | [H: forall x, in_bigrammar_rng (Map fi1 g) _ -> _ |- _] =>
+        guess (fst fi1 v) H; localsimpl
+    end.
+  - remember_head_in_hyp as sf.
+    destruct sf; try discriminate.
+    match goal with
+      | [H: forall V W, _ -> _ -> fst fi1 V = W |- _] => 
+        erewrite H in * by eauto; crush
+    end.
+Qed.
+
+Lemma pretty_print_corr2: forall t (g:bigrammar t) (v:interp t) s,
+  pretty_print g v = Some s -> wf_grammar g -> in_bigrammar g s v.
+Proof. 
+  induction g; try (localsimpl; fail).
+
+  - (* Cat *)
+    localsimpl.
+    destruct v. simpl in *.
+    remember_head_in_hyp as e1; destruct e1; try discriminate.
+    remember_head_in_hyp as e2; destruct e2; try discriminate.
+    crush.
+
+  - (* Alt *)
+    localsimpl.
+    destruct v; eauto using InAlt_l, InAlt_r.
+
+  (* Case "Star". *)
+  (*   induction v; simprover. *)
+  (*   remember_head_in_hyp as e1; destruct e1; try discriminate. *)
+  (*   destruct l; try discriminate. *)
+  (*   remember_head_in_hyp as e2; destruct e2; try discriminate. *)
+  (*   eapply InStar_cons; (eauto || simprover). *)
+
+  - (* Map. *)
+    localsimpl.
+    remember_head_in_hyp as e1; destruct e1; try discriminate.
+    guess v H2. crush.
+Qed.
+
+Lemma pretty_print_corr1: forall t (g:bigrammar t) (v:interp t) s,
+  in_bigrammar g s v -> wf_grammar g -> exists s', pretty_print g v = Some s'.
+Proof. 
+  induction g; try (localsimpl; fail).
+
+  - (* Cat *)
+    localsimpl. crush_hyp.
+    
+  (* Case "Star". *)
+  (*   induction v. simprover; eauto. *)
+  (*   intros. *)
+  (*   in_inv. *)
+  (*   apply StarInv in H. *)
+  (*   simprover. *)
+  (*   assert (exists s1, pretty_print g x0 = Some s1); eauto. *)
+  (*   assert (exists s2, pretty_print (Star g) x2 = Some s2); eauto. *)
+  (*   simprover. *)
+  (*   eexists. *)
+  (*   simprover. *)
+  (*   eauto. rewrite H3. *)
+  (*   ??? *)
+  
+  - (* Map *)
+    localsimpl. guess x H1. crush.
+Qed.
+
+
+      
